## Linear Equation

### Definition

Given a linear operator $L$, an equation having the form

$$
L(\boldsymbol(x)) = \boldsymbol{h}
$$

is a linear equation.

### Homogeneous Linear Equation

A linear equation $L(\boldsymbol{x}) = \boldsymbol{h}$ is homogeneous if and only if $\boldsymbol{h} \equiv \boldsymbol{0}$

### Superposition Principle

#### Theorem

Given a homogeneous linear equation

$$
L(\boldsymbol{x}) = \boldsymbol{0}
$$

if $\boldsymbol{x}_{1}$ and $\boldsymbol{x}_{2}$ are both its solutions, their linear combinations are also the solutions of the equation.

#### Proof

Let $a$ and $b$ be two scalars. Applying the property of linear operator,

$$
L(a\boldsymbol{x}_{1} + b\boldsymbol{x}_{2}) = aL(\boldsymbol{x}_{1}) + bL( \boldsymbol{x}_{2}) = 0
$$

so $a\boldsymbol{x}_{1} + b\boldsymbol{x}_{2}$ is a solution of $L(\boldsymbol{x}) = \boldsymbol{0}$.

### Non-homogeneous Principle

#### Theorem

Given a non-homogeneous linear equation

$$
L(\boldsymbol{x}) = \boldsymbol{h}
$$

if $\boldsymbol{x}_{p}$ is a solution of it and $\boldsymbol{x}_{h}$ is a solution of the corresponding homogeneous equation (i.e. $L(\boldsymbol{x}) = \boldsymbol{0}$), then $\boldsymbol{x}_{p} + \boldsymbol{x}_{h}$ is also a solution of the non-homogeneous equation.

#### Proof

Applying the property of linear operator,

$$
L(\boldsymbol{x}_{p} + \boldsymbol{x}_{h}) = L(\boldsymbol{x}_{p}) + L(\boldsymbol{x}_{h}) = \boldsymbol{h} + 0 = \boldsymbol{h}
$$

so $\boldsymbol{x}_{p} + \boldsymbol{x}_{h}$ is a solution of $L(\boldsymbol{x}) = \boldsymbol{h}$.

